Added compress functions. Needs to be verified
The compress function tries to use the Run-length encoding algorithm, returning, for example, the string \A6\B4 when the input string is AAAAAABBBB

Project/compression.dfy
@@ -1,3 +1,7 @@
+
+newtype {:nativeType "uint"}   uint32 = i:int | 0 <= i < 0x100000000
+newtype {:nativeType "byte"}   byte   = b:int | 0 <= b < 256
+
 /*method Main(args: array<seq<char>>) {
     var i := 0;
     while(i < args.Length)
@@ -10,6 +14,12 @@
 }*/
 
 //type T = int // for demo purposes, but could be another type
+
+function method ToString(n: int) : string 
+    requires n >= 0
+{   
+    if n == 0 then "" else ToString(n / 10) + [(n % 10) as char]
+}
  
 class {:autocontracts} Compression {
 
@@ -17,22 +27,69 @@ class {:autocontracts} Compression {
     {}*/
     
  
-    /*constructor () 
-    {}*/
+    constructor () 
+    {}
  
-    method compress(s: string) returns (comp_s: string) 
-        ensures s == decompress(comp_s);
+    method getStringPortionCMP(c: char, occ: int) returns (s: string) 
+        requires occ > 0
+        ensures occ > 3 ==> |s| == 2 + |ToString(occ)|
+        ensures occ <= 3 ==> |s| == occ
+    {
+        s := "";
+
+        if occ > 3 {
+            var tmp_s :=  ToString(occ);
+            s := ['\\'] + [c] + tmp_s;
+        } else {
+            var j := 0;
+            while j < occ 
+                decreases occ - j
+                invariant 0 <= j <= occ
+                invariant |s| == j
+            {
+                s := s + [c];
+                j := j + 1;
+            }
+        }
+    }
+    method compress(s: string) returns (comp_s: string)
+        requires |s| > 0
+        ensures |s| >= |comp_s|
     {
         comp_s := "";
+        var cnt_occur : int := 1;
+        var cur_char : char := s[0];
 
-        return comp_s;
+        var i := 1; // iterates through the string
+        
+        while i < |s|
+            decreases |s| - i
+            invariant 1 <= i <= |s|
+            invariant cur_char in s 
+            invariant 1 <= cnt_occur <= |s|
+        {
+            if s[i] == cur_char {
+                cnt_occur := cnt_occur + 1;
+            } else {
+                var tmp_s := getStringPortionCMP(cur_char, cnt_occur);
+                comp_s := comp_s + tmp_s;
+
+                cur_char := s[i];
+                cnt_occur := 1;
+            }
+
+            i := i + 1;
+        }
+
+        var tmp_s := getStringPortionCMP(cur_char, cnt_occur);
+        comp_s := comp_s + tmp_s;
     }
 
-    method decompress(s: string) returns (decomp_s: string) 
+    method decompress(s: string)  returns (decomp_s: string)
+        requires |s| > 0
+        ensures |s| <= |decomp_s|
     {
         decomp_s := "";
-
-        return decomp_s;
     }
 
  
@@ -41,5 +98,11 @@ class {:autocontracts} Compression {
 // A simple test scenario.
 method Main()
 {
-
+    var compression := new Compression();
+    var s := "aaabbbbbbccc";
+    var comp := compression.compress(s);
+    print comp;
+    assert multiset(s) == multiset("aaa\\b6ccc");
+    var decomp := compression.decompress(comp);
+    assert decomp == s;
 }
